Foundation/Modal/Maximal/Unprovability.lean
@@ -38,7 +38,7 @@ end Ver
 
 namespace K4
 
-lemma provable_trivTranslated_Cl : (Logic.K4) ⊢! φ → (Hilbert.Cl) ⊢! φᵀ.toPropFormula := by
+lemma provable_trivTranslated_Cl : (Logic.K4) ⊢! φ → Logic.Cl ⊢! φᵀ.toPropFormula := by
   intro h;
   apply Logic.Triv.iff_provable_Cl.mp;
   apply WeakerThan.pbl h;
@@ -64,7 +64,7 @@ instance : Logic.K4 ⪱ Logic.GL := by
 
 namespace GL
 
-lemma provable_verTranslated_Cl : (Logic.GL) ⊢! φ → (Hilbert.Cl) ⊢! φⱽ.toPropFormula := by
+lemma provable_verTranslated_Cl : (Logic.GL) ⊢! φ → Logic.Cl ⊢! φⱽ.toPropFormula := by
   intro h;
   induction h with
     | maxm a =>
