Foundation/Propositional/Logic/Letterless_Int_Cl.lean
@@ -21,7 +21,7 @@ theorem iff_letterless_Int_Cl {φ : Formula ℕ} (hφ : φ.letterless) : φ ∈ 
     have : Modal.Logic.S4 ⊢! ◇φᵍ := Modal.Logic.iff_provable_Cl_provable_dia_gS4.mp h;
     have : Modal.Logic.Triv ⊢! ◇φᵍ := WeakerThan.pbl this;
     have : Modal.Logic.Triv ⊢! φᵍ := diaT'! this;
-    have : Hilbert.Cl ⊢! φᵍᵀ.toPropFormula _ := Modal.Logic.Triv.iff_provable_Cl.mp this;
+    have : Logic.Cl ⊢! φᵍᵀ.toPropFormula _ := Modal.Logic.Triv.iff_provable_Cl.mp this;
     have : Semantics.Valid (ClassicalSemantics.Valuation ℕ) (φᵍᵀ.toPropFormula _) := Hilbert.Cl.soundness this;
     have : Modal.Logic.KD ⊢! φᵍ := Modal.Logic.provable_KD_of_classical_tautology (Formula.goedelTranslate.letterless hφ) this;
     have : Modal.Logic.S4 ⊢! φᵍ := WeakerThan.pbl this;
